Semantic/ModalCapybara/Syntax/Exp.lean
@@ -35,11 +35,13 @@ def Exp.rename : Exp s1 -> Rename s1 s2 -> Exp s2
 | .abs cs T e, f => .abs (cs.rename f) (T.rename f) (e.rename (f.lift))
 | .tabs cs T e, f => .tabs (cs.rename f) (T.rename f) (e.rename (f.lift))
 | .cabs cs m e, f => .cabs (cs.rename f) m (e.rename (f.lift))
+| .boxed Ψ e, f => .boxed (Ψ.rename f) (e.rename f)
 | .reader x, f => .reader (x.rename f)
 | .pack cs x, f => .pack (cs.rename f) (x.rename f)
 | .app x y, f => .app (x.rename f) (y.rename f)
 | .tapp x T, f => .tapp (x.rename f) (T.rename f)
 | .capp x cs, f => .capp (x.rename f) (cs.rename f)
+| .unwrap x, f => .unwrap (x.rename f)
 | .letin e1 e2, f => .letin (e1.rename f) (e2.rename (f.lift))
 | .unpack e1 e2, f => .unpack (e1.rename f) (e2.rename (f.lift.lift))
 | .unit, _ => .unit
@@ -55,6 +57,7 @@ inductive Exp.IsVal : Exp s -> Prop where
 | abs : Exp.IsVal (.abs cs T e)
 | tabs : Exp.IsVal (.tabs cs T e)
 | cabs : Exp.IsVal (.cabs cs m e)
+| boxed : Exp.IsVal (.boxed Ψ e)
 | pack : Exp.IsVal (.pack cs x)
 | reader : Exp.IsVal (.reader x)
 | unit : Exp.IsVal .unit
@@ -67,6 +70,7 @@ inductive Exp.IsSimpleVal : Exp s -> Prop where
 | abs : Exp.IsSimpleVal (.abs cs T e)
 | tabs : Exp.IsSimpleVal (.tabs cs T e)
 | cabs : Exp.IsSimpleVal (.cabs cs m e)
+| boxed : Exp.IsSimpleVal (.boxed Ψ e)
 | unit : Exp.IsSimpleVal .unit
 | btrue : Exp.IsSimpleVal .btrue
 | bfalse : Exp.IsSimpleVal .bfalse
@@ -97,7 +101,7 @@ def Exp.rename_id {e : Exp s} : e.rename (Rename.id) = e := by
     <;> try (solve
       | rfl
       | simp [Exp.rename, Ty.rename_id, PureTy.rename_id, Var.rename_id,
-              CaptureSet.rename_id, Rename.lift_id]
+              CaptureSet.rename_id, SepCtx.rename_id, Rename.lift_id]
         try aesop)
 
 /-- Renaming distributes over composition of renamings. -/
@@ -112,7 +116,7 @@ theorem Exp.rename_comp {e : Exp s1} {f : Rename s1 s2} {g : Rename s2 s3} :
     <;> try (solve
       | rfl
       | simp [Exp.rename, Ty.rename_comp, PureTy.rename_comp, Var.rename_comp,
-              CaptureSet.rename_comp, Rename.lift_comp]
+              CaptureSet.rename_comp, SepCtx.rename_comp, Rename.lift_comp]
         try aesop)
 
 /-- Weakening commutes with renaming under a binder. -/
@@ -137,11 +141,14 @@ inductive Exp.IsClosed : Exp s -> Prop where
     Exp.IsClosed (.tabs cs T e)
 | cabs : CaptureSet.IsClosed cs -> Exp.IsClosed e ->
     Exp.IsClosed (.cabs cs m e)
+| boxed : SepCtx.IsClosed Ψ -> Exp.IsClosed e ->
+    Exp.IsClosed (.boxed Ψ e)
 | reader : Var.IsClosed x -> Exp.IsClosed (.reader x)
 | pack : CaptureSet.IsClosed cs -> Var.IsClosed x -> Exp.IsClosed (.pack cs x)
 | app : Var.IsClosed x -> Var.IsClosed y -> Exp.IsClosed (.app x y)
 | tapp : Var.IsClosed x -> PureTy.IsClosed T -> Exp.IsClosed (.tapp x T)
 | capp : Var.IsClosed x -> CaptureSet.IsClosed cs -> Exp.IsClosed (.capp x cs)
+| unwrap : Var.IsClosed x -> Exp.IsClosed (.unwrap x)
 | letin : Exp.IsClosed e1 -> Exp.IsClosed e2 -> Exp.IsClosed (.letin e1 e2)
 | unpack : Exp.IsClosed e1 -> Exp.IsClosed e2 -> Exp.IsClosed (.unpack e1 e2)
 | unit : Exp.IsClosed .unit
